Refined Terminals & Open Any & Fix Choice

src/ASN1/ASN1.Base.fst
@@ -13,7 +13,6 @@ module U8 = FStar.UInt8
 module B = FStar.Bytes
 module Seq = FStar.Seq
 module List = FStar.List.Tot
-//module Set = FStar.Set
 
 // ASN.1 Identifier
 
@@ -32,7 +31,7 @@ type asn1_id_value_t = U32.t
 type asn1_id_t =
 | MK_ASN1_ID : c : asn1_id_class_t -> f : asn1_id_flag_t -> v : asn1_id_value_t -> asn1_id_t
 
-//TODO: constant tables
+//TODO: constant tables (Currently in X.509)
 
 //ASN.1 kinds and High-level types
 
@@ -58,9 +57,6 @@ type asn1_terminal_k : Type =
 type asn1_boolean_t = bool
 
 type asn1_integer_t = I32.t
-
-//Maybe we should encode more information for enum types
-// type asn1_enum_t = U32.t
 
 //Bitstring is represented as an array of bytes and 0~7 unused bits
 type asn1_bitstring_t = 
@@ -124,59 +120,10 @@ let rec asn1_terminal_t (k : asn1_terminal_k) : eqtype =
   | ASN1_GENERALIZEDTIME -> asn1_generalizedtime_t
   | ASN1_PREFIXED_TERMINAL _ k -> asn1_terminal_t k
 
-// Those two ways of implementation should be equivalent except for a layer of wrapper which is unnecessary
-
-(*
-type asn1_terminal_t : asn1_terminal_k -> Type =
-| Mk_ASN1_BOOLEAN : asn1_boolean_t -> asn1_terminal_t ASN1_BOOLEAN
-| Mk_ASN1_INTEGER : asn1_integer_t -> asn1_terminal_t ASN1_INTEGER
-| Mk_ASN1_ENUM : asn1_enum_t -> asn1_terminal_t ASN1_ENUM
-| Mk_ASN1_BITSTRING : asn1_bitstring_t -> asn1_terminal_t ASN1_BITSTRING
-| Mk_ASN1_OCTETSTRING : asn1_octetstring_t -> asn1_terminal_t ASN1_OCTETSTRING
-| Mk_ASN1_NULL : asn1_terminal_t ASN1_NULL
-| Mk_ASN1_OID : asn1_oid_t -> asn1_terminal_t ASN1_OID
-| Mk_ASN1_ROID : asn1_roid_t -> asn1_terminal_t ASN1_ROID
-| Mk_ASN1_TIME : asn1_time_t -> asn1_terminal_t ASN1_TIME
-
-let asn1_terminal_type_of (k : asn1_terminal_k) : Type =
-  match k with
-  | ASN1_BOOLEAN -> asn1_terminal_t ASN1_BOOLEAN
-  | ASN1_INTEGER -> asn1_terminal_t ASN1_INTEGER
-  | ASN1_ENUM -> asn1_terminal_t ASN1_ENUM
-  | ASN1_BITSTRING -> asn1_terminal_t ASN1_BITSTRING
-  | ASN1_OCTETSTRING -> asn1_terminal_t ASN1_OCTETSTRING
-  | ASN1_NULL -> asn1_terminal_t ASN1_NULL
-  | ASN1_OID -> asn1_terminal_t ASN1_OID
-  | ASN1_ROID -> asn1_terminal_t ASN1_ROID
-  | ASN1_TIME -> asn1_terminal_t ASN1_TIME
-*)
-
 type asn1_decorator : Type =
 | PLAIN
 | OPTION
 | DEFAULT
-
-(*
-and asn1_sequence_k : Set.set asn1_id_t -> Type =
-| ASN1_SEQUENCE : items : list ((s : Set.set asn1_id_t) & (asn1_decorated_k s)) ->
-                  pf : (asn1_sequence_k_wf items) ->
-                  asn1_sequence_k         
-| ASN1_SEQUENCE_NIL : asn1_sequence_k (Set.empty)
-| ASN1_SEQUENCE_CONS_PLAIN : #s : _ -> h : asn1_k s ->
-                             #s' : _ -> t : asn1_sequence_k s'->
-                             asn1_sequence_k s
-| ASN1_SEQUENCE_CONS_OPTIONAL : #s : _ -> h : asn1_k s ->
-                                #s' : _ -> t : asn1_sequence_k s' ->
-                                squash (Set.disjoint s s') ->
-                                asn1_sequence_k (Set.union s s')
-| ASN1_SEQUENCE_CONS_DEFAULT_TERMINAL : id : asn1_id_t ->
-                                        #k : asn1_terminal_k ->
-                                        defaultv : asn1_terminal_t k ->
-                                        #s : _ -> t : asn1_sequence_k s ->
-                                        squash (~(Set.mem id s)) ->
-                                        asn1_sequence_k (Set.union (Set.singleton id) s)
-*)
-
 
 let rec asn1_sequence_k_wf' (li : list ((Set.set asn1_id_t) & asn1_decorator)) (s : Set.set asn1_id_t) : Type =
   match li with
@@ -195,21 +142,22 @@ let my_as_set = Set.as_set
 
 noeq noextract
 type asn1_content_k : Type =
+| ASN1_RESTRICTED_TERMINAL : (k : asn1_terminal_k) -> (is_valid : (asn1_terminal_t k) -> bool) -> asn1_content_k
 | ASN1_TERMINAL : asn1_terminal_k -> asn1_content_k
-| ASN1_SEQUENCE : items : list (asn1_gen_item_k) -> 
-                  pf : squash (asn1_sequence_k_wf (List.map (fun x -> match x with |(| s, d, _ |) -> (s, d) ) items)) ->
-                  asn1_content_k
+| ASN1_SEQUENCE : asn1_gen_items_k -> asn1_content_k
 | ASN1_SEQUENCE_OF : #s : _ -> asn1_k s -> asn1_content_k
 //| ASN1_SET : #s : _ -> asn1_set_k s -> asn1_content_k
 | ASN1_SET_OF : #s : _ -> asn1_k s -> asn1_content_k
 | ASN1_PREFIXED : #s : _ -> asn1_k s -> asn1_content_k
 | ASN1_ANY_OID : asn1_id_t ->
-                 supported : list (asn1_oid_t * asn1_gen_item_k) -> 
-                 pf : squash ((Cons? supported) /\ List.noRepeats (List.map fst supported)) -> 
+                 supported : list (asn1_oid_t * asn1_gen_items_k) -> 
+                 fallback : option asn1_gen_items_k ->
+                 pf : squash (List.noRepeats (List.map fst supported)) -> 
                  asn1_content_k
 | ASN1_ANY_INTEGER : asn1_id_t ->
-                 supported : list (asn1_integer_t * asn1_gen_item_k) -> 
-                 pf : squash ((Cons? supported) /\ List.noRepeats (List.map fst supported)) -> 
+                 supported : list (asn1_integer_t * asn1_gen_items_k) -> 
+                 fallback : option asn1_gen_items_k ->
+                 pf : squash (List.noRepeats (List.map fst supported)) -> 
                  asn1_content_k
 
 // The complete ASN.1 kind is indexed by the set of valid first identifiers
@@ -217,15 +165,19 @@ type asn1_content_k : Type =
 and asn1_k : Set.set asn1_id_t -> Type =
 | ASN1_ILC : id : asn1_id_t -> asn1_content_k -> asn1_k (Set.singleton id)
 | ASN1_CHOICE_ILC : choices : list (asn1_id_t & asn1_content_k) -> 
-                    pf : squash ((Cons? choices) /\ (List.noRepeats (List.map fst choices))) -> 
+                    pf : squash (List.noRepeats (List.map fst choices)) -> 
                     asn1_k (my_as_set (List.map fst choices))
                     
 and asn1_decorated_k : Set.set asn1_id_t -> asn1_decorator -> Type =
 | ASN1_PLAIN_ILC : #s : _ -> k : asn1_k s -> asn1_decorated_k s PLAIN
 | ASN1_OPTION_ILC : #s : _ -> k : asn1_k s -> asn1_decorated_k s OPTION
 | ASN1_DEFAULT_TERMINAL : id : asn1_id_t -> #k : asn1_terminal_k -> defaultv : asn1_terminal_t k -> asn1_decorated_k (Set.singleton id) DEFAULT
+| ASN1_DEFAULT_RESTRICTED_TERMINAL : id : asn1_id_t -> #k : asn1_terminal_k -> is_valid : ((asn1_terminal_t k) -> bool) -> 
+                                     defaultv : asn1_terminal_t k {is_valid defaultv = true} -> asn1_decorated_k (Set.singleton id) DEFAULT
 
 and asn1_gen_item_k : Type = s : Set.set asn1_id_t & d : asn1_decorator & asn1_decorated_k s d
+
+and asn1_gen_items_k : Type = items : list (asn1_gen_item_k) & squash (asn1_sequence_k_wf (List.map (fun x -> match x with |(| s, d, _ |) -> (s, d) ) items))
 
 let mk_ASN1_GEN_ITEM (#s) (#d) (k : asn1_decorated_k s d) : asn1_gen_item_k =
   (| s, d, k |)
@@ -264,37 +216,51 @@ let idlookup_t (#key : eqtype) (id : key) (lc : list (key & Type)) :
     let _ = List.assoc_memP_none id lc in
     False 
 
+let idlookup_with_fallback_t_postcond (#key : eqtype) (id : key) (lc : list (key & Type)) (fb : Type) (t : Type) : GTot Type0
+= (t << lc \/ t == fb)
+
+let idlookup_with_fallback_t (#key : eqtype) (id : key) (lc : list (key & Type)) (fb : Type) :
+  Pure Type
+  (requires True)
+  (ensures fun t -> idlookup_with_fallback_t_postcond id lc fb t)
+= let _ = List.assoc_mem id lc in
+  let res = List.assoc id lc in
+  match res with
+  | Some t -> 
+    let _ = List.assoc_memP_some id t lc in
+    let _ = assoc_slt lc id in
+    t  
+  | None -> 
+    let _ = List.assoc_memP_none id lc in
+    fb
+
 let make_gen_choice_type (#key : eqtype) (lc : list (key & Type)) = (id : key) & (idlookup_t id lc)
 
-(*
-noeq noextract
-type asn1_content_k : Type =
-| ASN1_TERMINAL : asn1_terminal_k -> asn1_content_k
-| ASN1_SEQUENCE : items : list (asn1_gen_item_k) -> 
-                  pf : (asn1_sequence_k_wf (List.map (fun x -> match x with |(| s, d, _ |) -> (s, d) ) items)) ->
-                  asn1_content_k
-| ASN1_SEQUENCE_OF : #s : _ -> asn1_k s -> asn1_content_k
-//| ASN1_SET : #s : _ -> asn1_set_k s -> asn1_content_k
-| ASN1_SET_OF : #s : _ -> asn1_k s -> asn1_content_k
-| ASN1_PREFIXED : #s : _ -> asn1_k s -> asn1_content_k
-*)
+let make_gen_choice_type_with_fallback (#key : eqtype) (lc : list (key & Type)) (fb : Type) = (id : key) & (idlookup_with_fallback_t id lc fb)
 
 let rec asn1_content_t (k : asn1_content_k) : Tot Type (decreases k) =
   match k with
+  | ASN1_RESTRICTED_TERMINAL k' is_valid -> parse_filter_refine is_valid
   | ASN1_TERMINAL k' -> asn1_terminal_t k'
-  | ASN1_SEQUENCE items pf -> asn1_sequence_t items
+  | ASN1_SEQUENCE gitems -> asn1_sequence_t (dfst gitems)
   | ASN1_SEQUENCE_OF k' ->  list (asn1_t k')
   | ASN1_SET_OF k' -> asn1_t k'
   | ASN1_PREFIXED k' -> asn1_t k'
-  | ASN1_ANY_OID id ls pf -> make_gen_choice_type (asn1_any_t asn1_oid_t ls)
-  | ASN1_ANY_INTEGER id ls pf -> make_gen_choice_type (asn1_any_t asn1_integer_t ls)
+  | ASN1_ANY_OID id ls ofb pf -> 
+    (match ofb with
+    | None -> make_gen_choice_type (asn1_any_t asn1_oid_t ls)
+    | Some fb -> make_gen_choice_type_with_fallback (asn1_any_t asn1_oid_t ls) (asn1_sequence_t (dfst fb)))
+  | ASN1_ANY_INTEGER id ls ofb pf ->
+    (match ofb with
+    | None -> make_gen_choice_type (asn1_any_t asn1_integer_t ls)
+    | Some fb -> make_gen_choice_type_with_fallback (asn1_any_t asn1_integer_t ls) (asn1_sequence_t (dfst fb)))
 
-and asn1_any_t (t : eqtype) (ls : list (t * asn1_gen_item_k)) : Tot (list (t & Type)) (decreases ls) =
+and asn1_any_t (t : eqtype) (ls : list (t * asn1_gen_items_k)) : Tot (list (t & Type)) (decreases ls) =
   match ls with
   | [] -> [] 
   | h :: tl -> 
     let (x, y) = h in
-    (x, asn1_decorated_t y) :: (asn1_any_t t tl)
+    (x, asn1_sequence_t (dfst y)) :: (asn1_any_t t tl)
 
 and asn1_lc_t (lc : list (asn1_id_t & asn1_content_k)) : Tot (list (asn1_id_t & Type)) (decreases lc) =
   match lc with
@@ -315,6 +281,7 @@ and asn1_decorated_t (item : asn1_gen_item_k) : Tot Type =
                     | ASN1_PLAIN_ILC k -> asn1_t k
                     | ASN1_OPTION_ILC k -> (option (asn1_t k)) 
                     | ASN1_DEFAULT_TERMINAL id defv -> (default_tv defv)
+                    | ASN1_DEFAULT_RESTRICTED_TERMINAL id #k is_valid defv -> default_tv #(parse_filter_refine is_valid) defv
 
 and asn1_sequence_t (items : list asn1_gen_item_k) : Tot Type (decreases items) =
   match items with
@@ -331,6 +298,7 @@ let asn1_decorated_pure_t (item : asn1_gen_item_k) : Type =
                      | ASN1_PLAIN_ILC k -> asn1_t k
                      | ASN1_OPTION_ILC k -> asn1_t k
                      | ASN1_DEFAULT_TERMINAL _ #k _ -> asn1_terminal_t k 
+                     | ASN1_DEFAULT_RESTRICTED_TERMINAL _ #k is_valid _ -> parse_filter_refine is_valid
 
 type asn1_strong_parser_kind : parser_kind = {
   parser_kind_metadata = None;
@@ -360,65 +328,3 @@ type gen_decorated_parser_twin =
 -> fp : (asn1_id_t -> asn1_strong_parser (asn1_decorated_pure_t d)) {and_then_cases_injective fp} ->
 gen_decorated_parser_twin
 
-(*
-
-noeq
-type gen_parser =
-| Mkgenparser : (k : parser_kind) -> (t : Type) -> (p : parser k t) -> gen_parser
-
-noeq
-type gen_decorated_parser_twin =
-| Mkgendcparser : (d : asn1_gen_item_k) -> (k : parser_kind) -> (p : parser k (asn1_decorated_pure_t d)) -> (k' : parser_kind) -> fp : (asn1_id_t -> parser k' (asn1_decorated_pure_t d)) {and_then_cases_injective fp} -> gen_decorated_parser_twin
-
-*)
-
-(*
-noeq
-type asn1_content_t : asn1_content_k -> Type =
-| Mk_ASN1_TERMINAL : k : asn1_terminal_k -> asn1_terminal_t k -> asn1_content_t (ASN1_TERMINAL k)
-| Mk_ASN1_SEQUENCE : #s : _ -> #k : asn1_sequence_k s -> asn1_content_t (ASN1_SEQUENCE k)
-| Mk_ASN1_SEQUENCE_OF : #s : _ -> #k : asn1_k s -> sv : Seq.seq (asn1_t k) -> asn1_content_t (ASN1_SEQUENCE_OF k)
-| MK_ASN1_SINGLETON_SET_OF : #s : _ -> #k : asn1_k s -> v : asn1_t k -> asn1_content_t (ASN1_SET_OF k)
-| Mk_ASN1_PREFIXED : #s : _ -> #k : asn1_k s -> v : asn1_t k -> asn1_content_t (ASN1_PREFIXED k)
-
-and asn1_lc_t : asn1_content_k -> Type =
-| Mk_ASN1_LC : #k : _ -> asn1_content_t k -> asn1_lc_t k
-
-and asn1_t : #s : _ -> asn1_k s -> Type =
-| Mk_ASN1_ILC : id : asn1_id_t -> #k : _ -> asn1_lc_t k -> asn1_t (ASN1_ILC id k)
-| Mk_ASN1_CHOICE_ILC : #s : _ -> #k : asn1_choice_k s -> asn1_choice_t k -> asn1_t (ASN1_CHOICE_ILC k)
-
-and asn1_choice_t : #s : _ -> asn1_choice_k s -> Type =
-| Mk_ASN1_CHOICE_SINGLETON : #s : _ -> #k : asn1_k s -> asn1_t k -> asn1_choice_t (ASN1_CHOICE_SINGLETON k)
-| Mk_ASN1_CHOICE_CONS_THIS : #s : _ -> #k : asn1_k s -> asn1_t k -> 
-                             #s' : _ -> k' : asn1_choice_k s' ->
-                             #pf : squash (Set.disjoint s s') ->
-                             asn1_choice_t #(Set.union s s') (ASN1_CHOICE_CONS k k' pf)
-| Mk_ASN1_CHOICE_CONS_THAT : #s : _ -> k : asn1_k s ->
-                             #s' : _ -> #k' : asn1_choice_k s' -> asn1_choice_t k' ->
-                             #pf : squash (Set.disjoint s s') ->
-                             asn1_choice_t #(Set.union s s') (ASN1_CHOICE_CONS k k' pf)
-
-and optional_asn1_t (#s : _) (k : asn1_k s) =
-| Mk_ASN1_NONE : optional_asn1_t k
-| Mk_ASN1_SOME : v : (asn1_t k) -> optional_asn1_t k
-
-and default_asn1_t (#k : asn1_terminal_k) (v : asn1_terminal_t k) =
-| Mk_ASN1_DEFAULT : default_asn1_t v
-| Mk_ASN1_NON_DEFAULT : v' : asn1_terminal_t k -> squash (~(v' = v)) -> default_asn1_t v 
-
-and asn1_sequence_t : #s : _ -> asn1_sequence_k s -> Type =
-| Mk_ASN1_SEQUENCE_NIL : asn1_sequence_t (ASN1_SEQUENCE_NIL)
-| Mk_ASN1_SEQUENCE_CONS_PLAIN : #s : _ -> #k : asn1_k s -> h : asn1_t k ->
-                                #s' : _ -> #k' : asn1_sequence_k s' -> t : asn1_sequence_t k' ->
-                                asn1_sequence_t (ASN1_SEQUENCE_CONS_PLAIN k k')
-| Mk_ASN1_SEQUENCE_CONS_OPTIONAL : #s : _ -> #k : asn1_k s -> h : optional_asn1_t k ->
-                                   #s' : _ -> #k' : asn1_sequence_k s' -> t : asn1_sequence_t k' ->
-                                   #pf : squash (Set.disjoint s s') ->
-                                   asn1_sequence_t (ASN1_SEQUENCE_CONS_OPTIONAL k k' pf)
-| Mk_ASN1_SEQUENCE_CONS_DEFAULT : #id : asn1_id_t -> #k : asn1_terminal_k -> #defaultv : asn1_terminal_t k -> v : default_asn1_t defaultv ->
-                                  #s' : _ -> #k' : asn1_sequence_k s' -> t : asn1_sequence_t k' ->
-                                  #pf : squash (~(Set.mem id s')) ->
-                                  asn1_sequence_t (ASN1_SEQUENCE_CONS_DEFAULT_TERMINAL id defaultv k' pf)
-
-*)
