src/ASN1/ASN1.Spec.Any.fst
@@ -14,49 +14,128 @@ module List = FStar.List.Tot
 
 let rec make_gen_choice_weak_payload_parser
   (#t : eqtype)
-  (lc : list (t & (gen_parser asn1_weak_parser_kind)) {Cons? lc})
+  (lc : list (t & (gen_parser asn1_weak_parser_kind)))
 //  (pf : List.noRepeats (List.map fst lc))
   : Tot (id : t -> asn1_weak_parser 
                   (refine_with_tag (project_tags lc) id))
 = fun id ->
   match lc with
+  | [] -> fail_parser _ _
   | hd :: tl ->
     let (id', gp) = hd in
     if (id = id') then
       let p = (Mkgenparser?.p gp) in 
       parse_synth p (attach_tag lc id)
     else      
-      (match tl with
-      | nil -> fail_parser asn1_weak_parser_kind (refine_with_tag (project_tags lc) id)
-      | _ -> make_gen_choice_weak_payload_parser tl id)
+      parse_synth (make_gen_choice_weak_payload_parser tl id) (fun x -> lemma_choice_cast (fst hd, Mkgenparser?.t (snd hd)) (extract_types tl) id x)
 
 let make_gen_choice_weak_parser
   (#t : eqtype)
   (#k : parser_kind)
   (p : parser k t)
-  (lc : list (t & (gen_parser asn1_weak_parser_kind)) {Cons? lc})
+  (lc : list (t & (gen_parser asn1_weak_parser_kind)))
   //(pf : List.noRepeats (List.map fst lc))
   : parser (and_then_kind k asn1_weak_parser_kind) (make_gen_choice_type (extract_types lc))
 = parse_tagged_union p (tag_of_gen_choice_type (extract_types lc)) (make_gen_choice_weak_payload_parser lc)
 
-let make_asn1_any_OIDU32_parser
+let tag_of_gen_choice_type_with_fallback (#key : eqtype) (lc : list (key & Type)) (fb : Type) : make_gen_choice_type_with_fallback lc fb -> Tot key = dfst
+
+let project_tags_with_fallback (#t : eqtype) (#k : parser_kind) (lc : list (t & (gen_parser k))) (fb : gen_parser k) =
+tag_of_gen_choice_type_with_fallback (extract_types lc) (Mkgenparser?.t fb)
+
+let attach_tag_with_fallback (#t : eqtype) (#k : parser_kind) (lc : list (t & (gen_parser k))) (fb : gen_parser k) (id : t) (x :  idlookup_with_fallback_t id (extract_types lc) (Mkgenparser?.t fb)) : 
+  (refine_with_tag (project_tags_with_fallback lc fb) id)
+= Mkdtuple2 id x
+
+let lemma_choice_with_fallback_cast
+  (#key : eqtype)
+  (hd : key & Type)
+  (tl : list (key & Type))
+  (fb : Type)
+  (id : key)
+  (ret : refine_with_tag (tag_of_gen_choice_type_with_fallback tl fb) id)
+: Pure (refine_with_tag (tag_of_gen_choice_type_with_fallback (hd :: tl) fb) id)
+  (requires id <> (fst hd))
+  (ensures (fun _ -> True))
+= let (|id', v|) = ret in
+  (|id', v|)
+
+let rec make_gen_choice_with_fallback_weak_payload_parser
+  (#t : eqtype)
+  (lc : list (t & (gen_parser asn1_weak_parser_kind)))
+  (fb : gen_parser asn1_weak_parser_kind)
+//  (pf : List.noRepeats (List.map fst lc))
+  : Tot (id : t -> asn1_weak_parser 
+                  (refine_with_tag (project_tags_with_fallback lc fb) id))
+= fun id ->
+  match lc with
+  | [] ->
+    assert (lc == []);
+    let _ = List.map_lemma (fun x -> (fst x, Mkgenparser?.t (snd x))) lc in
+    assert (extract_types lc == []);
+    parse_synth (Mkgenparser?.p fb) (attach_tag_with_fallback lc fb id)
+  | hd :: tl ->
+    let (id', gp) = hd in
+    if (id = id') then
+      let p = (Mkgenparser?.p gp) in 
+      parse_synth p (attach_tag_with_fallback lc fb id)
+    else      
+      parse_synth (make_gen_choice_with_fallback_weak_payload_parser tl fb id) (fun x -> lemma_choice_with_fallback_cast (fst hd, Mkgenparser?.t (snd hd)) (extract_types tl) (Mkgenparser?.t fb) id x)
+
+let make_gen_choice_with_fallback_weak_parser
+  (#t : eqtype)
+  (#k : parser_kind)
+  (p : parser k t)
+  (lc : list (t & (gen_parser asn1_weak_parser_kind)))
+  (fb : gen_parser asn1_weak_parser_kind)
+  //(pf : List.noRepeats (List.map fst lc))
+  : parser (and_then_kind k asn1_weak_parser_kind) (make_gen_choice_type_with_fallback (extract_types lc) (Mkgenparser?.t fb))
+= parse_tagged_union p (tag_of_gen_choice_type_with_fallback (extract_types lc) (Mkgenparser?.t fb)) (make_gen_choice_with_fallback_weak_payload_parser lc fb)
+
+let make_asn1_closed_any_OIDU32_parser
   (id : asn1_id_t)
-  (ls : list (asn1_oid_t * asn1_gen_item_k))
-  (pf : squash((Cons? ls) /\ (List.noRepeats (List.map fst ls))))
+  (ls : list (asn1_oid_t * asn1_gen_items_k))
+  (pf : squash((List.noRepeats (List.map fst ls))))
   (k : asn1_content_k)
   (lp : list (asn1_oid_t & (gen_parser asn1_weak_parser_kind)))
 : Pure (asn1_weak_parser (asn1_content_t k))
-  (requires ((k == ASN1_ANY_OID id ls pf) /\ (asn1_any_t asn1_oid_t ls == extract_types lp)))
+  (requires ((k == ASN1_ANY_OID id ls None pf) /\ (asn1_any_t asn1_oid_t ls == extract_types lp)))
   (ensures fun _ -> True)
 = weaken asn1_weak_parser_kind (make_gen_choice_weak_parser (parse_asn1_ILC id #(ASN1_TERMINAL ASN1_OID) parse_asn1_OIDU32) lp)
 
-let make_asn1_any_INTEGER_parser
+let make_asn1_closed_any_INTEGER_parser
   (id : asn1_id_t)
-  (ls : list (asn1_integer_t * asn1_gen_item_k))
-  (pf : squash((Cons? ls) /\ (List.noRepeats (List.map fst ls))))
+  (ls : list (asn1_integer_t * asn1_gen_items_k))
+  (pf : squash(List.noRepeats (List.map fst ls)))
   (k : asn1_content_k)
   (lp : list (asn1_integer_t & (gen_parser asn1_weak_parser_kind)))
 : Pure (asn1_weak_parser (asn1_content_t k))
-  (requires ((k == ASN1_ANY_INTEGER id ls pf) /\ (asn1_any_t asn1_integer_t ls == extract_types lp)))
+  (requires ((k == ASN1_ANY_INTEGER id ls None pf) /\ (asn1_any_t asn1_integer_t ls == extract_types lp)))
   (ensures fun _ -> True)
 = weaken asn1_weak_parser_kind (make_gen_choice_weak_parser (parse_asn1_ILC id #(ASN1_TERMINAL ASN1_INTEGER) (weaken _ parse_untagged_int32)) lp)
+
+let make_asn1_open_any_OIDU32_parser
+  (id : asn1_id_t)
+  (ls : list (asn1_oid_t * asn1_gen_items_k))
+  (fbk : asn1_gen_items_k)
+  (fbp : asn1_weak_parser (asn1_sequence_t (dfst fbk)))
+  (pf : squash((List.noRepeats (List.map fst ls))))
+  (k : asn1_content_k)
+  (lp : list (asn1_oid_t & (gen_parser asn1_weak_parser_kind)))
+: Pure (asn1_weak_parser (asn1_content_t k))
+  (requires ((k == ASN1_ANY_OID id ls (Some fbk) pf) /\ (asn1_any_t asn1_oid_t ls == extract_types lp)))
+  (ensures fun _ -> True)
+= weaken asn1_weak_parser_kind (make_gen_choice_with_fallback_weak_parser (parse_asn1_ILC id #(ASN1_TERMINAL ASN1_OID) parse_asn1_OIDU32) lp (Mkgenparser _ fbp))
+
+let make_asn1_open_any_INTEGER_parser
+  (id : asn1_id_t)
+  (ls : list (asn1_integer_t * asn1_gen_items_k))
+  (fbk : asn1_gen_items_k)
+  (fbp : asn1_weak_parser (asn1_sequence_t (dfst fbk)))
+  (pf : squash((List.noRepeats (List.map fst ls))))
+  (k : asn1_content_k)
+  (lp : list (asn1_integer_t & (gen_parser asn1_weak_parser_kind)))
+: Pure (asn1_weak_parser (asn1_content_t k))
+  (requires ((k == ASN1_ANY_INTEGER id ls (Some fbk) pf) /\ (asn1_any_t asn1_integer_t ls == extract_types lp)))
+  (ensures fun _ -> True)
+= weaken asn1_weak_parser_kind (make_gen_choice_with_fallback_weak_parser (parse_asn1_ILC id #(ASN1_TERMINAL ASN1_INTEGER) (weaken _ parse_untagged_int32)) lp (Mkgenparser _ fbp))
