src/ASN1/ASN1.Spec.Sequence.fst
@@ -21,6 +21,7 @@ let generate_defaultable_item (item : gen_decorated_parser_twin) :
                        | ASN1_PLAIN_ILC k -> None
                        | ASN1_OPTION_ILC k -> Some (None #(asn1_t k)) 
                        | ASN1_DEFAULT_TERMINAL id #k defv -> Some (Default #(asn1_terminal_t k) #defv)
+                       | ASN1_DEFAULT_RESTRICTED_TERMINAL id #k is_valid defv -> Some (Default #(asn1_decorated_pure_t (Mkgendcparser?.d item)) #defv)
 
 let rec generate_defaultable_items (itemtwins : list (gen_decorated_parser_twin)) :
   Tot (option (asn1_sequence_t (List.map (Mkgendcparser?.d) itemtwins)))
@@ -50,6 +51,15 @@ let parse_asn1_sequence_item_twin (item : gen_decorated_parser_twin) :
                     (defaultv_filter defaultv))
                     `parse_synth`
                     (defaultv_synth defaultv))
+           | ASN1_DEFAULT_RESTRICTED_TERMINAL _ is_valid defaultv -> fun id ->
+                    ((((fp id)
+                    `parse_filter`
+                    is_valid)
+                    `parse_filter`
+                    (defaultv_filter #(asn1_decorated_pure_t d) defaultv))
+                    `parse_synth`
+                    (defaultv_synth #(asn1_decorated_pure_t d) defaultv))
+
 
 let parse_asn1_sequence_item_twin_nondefault
   (item : gen_decorated_parser_twin)
@@ -78,6 +88,14 @@ let parse_asn1_sequence_item_twin_nondefault
            | Some (v, _) -> 
              let _ = parse_synth_eq ((fp id) `parse_filter` (defaultv_filter defaultv)) (defaultv_synth defaultv) input in
              ())
+        | ASN1_DEFAULT_RESTRICTED_TERMINAL _ is_valid defaultv ->
+          let defv = generate_defaultable_item item in
+          (match parse p input with
+           | None -> ()
+           | Some (v, _) -> 
+             let _ = parse_synth_eq (((fp id) `parse_filter` is_valid) `parse_filter` (defaultv_filter #(asn1_decorated_pure_t d) defaultv)) (defaultv_synth  #(asn1_decorated_pure_t d) defaultv) input in
+             ())
+
 
 let and_then_cases_injective_some
   (#t: Type)
@@ -153,6 +171,18 @@ let parse_asn1_sequence_item_twin_cases_injective
               parse_synth_eq ((fp id2) `parse_filter` (defaultv_filter defaultv)) (defaultv_synth defaultv) b2;
               parse_filter_eq (fp id1) (defaultv_filter defaultv) b1;
               parse_filter_eq (fp id2) (defaultv_filter defaultv) b2;
+              and_then_cases_injective_elim fp id1 id2 b1 b2
+          )
+        | ASN1_DEFAULT_RESTRICTED_TERMINAL _ is_valid defaultv ->
+          let p = parse_asn1_sequence_item_twin item in
+          and_then_cases_injective_intro p (
+            fun id1 id2 b1 b2 ->
+              parse_synth_eq (((fp id1) `parse_filter` is_valid) `parse_filter` (defaultv_filter #(asn1_decorated_pure_t d) defaultv)) (defaultv_synth #(asn1_decorated_pure_t d) defaultv) b1;
+              parse_synth_eq (((fp id2) `parse_filter` is_valid) `parse_filter` (defaultv_filter #(asn1_decorated_pure_t d) defaultv)) (defaultv_synth #(asn1_decorated_pure_t d) defaultv) b2;
+              parse_filter_eq ((fp id1) `parse_filter` is_valid) (defaultv_filter #(asn1_decorated_pure_t d) defaultv) b1;
+              parse_filter_eq ((fp id2) `parse_filter` is_valid) (defaultv_filter #(asn1_decorated_pure_t d) defaultv) b2;
+              parse_filter_eq (fp id1) is_valid b1;
+              parse_filter_eq (fp id2) is_valid b2;
               and_then_cases_injective_elim fp id1 id2 b1 b2
           )
   
